Veritas.Merkle.fsti
@@ -84,6 +84,16 @@ val addr_to_merkle_leaf (a:addr): Tot merkle_leaf_addr
 (* Inverse of addr_to_merkle_leaf *)
 val merkle_leaf_to_addr (ma:merkle_leaf_addr): Tot (a:addr{addr_to_merkle_leaf a = ma})
 
+val lemma_addr_merkle_inv (a:addr):
+  Lemma (merkle_leaf_to_addr (addr_to_merkle_leaf a) = a)
+
+val lemma_merkle_equal_implies_addr_equal (a1:addr) (a2:addr):
+  Lemma (requires (addr_to_merkle_leaf a1 = addr_to_merkle_leaf a2))
+        (ensures (a1 = a2))
+
+val lemma_addr_equal_implies_merkle_equal (m1:merkle_leaf_addr) (m2:merkle_leaf_addr):
+  Lemma (requires (merkle_leaf_to_addr m1 = merkle_leaf_to_addr m2))
+        (ensures (m1 = m2))
 (*
  * merklefn: compute the merkle tree value at each node
  * of the merkle tree
